code/ecdsap256/Hacl.Impl.P256.SolinasReduction.fst
@@ -5,8 +5,6 @@ open FStar.HyperStack
 module ST = FStar.HyperStack.ST
 
 open FStar.Mul
-open FStar.Math.Lemmas
-open FStar.Math.Lib
 module BV = FStar.BitVector
 module Seq = FStar.Seq
 
@@ -14,9 +12,12 @@ open Lib.IntTypes
 open Lib.Buffer
 
 open Spec.P256.Constants
+open Hacl.Spec.P256.SolinasReduction.Lemmas
+
+open Hacl.Impl.P256.Bignum
 open Hacl.Impl.P256.Field
 
-#reset-options "--fuel 0 --ifuel 0 --z3rlimit 50"
+#reset-options "--z3rlimit 50 --fuel 0 --ifuel 0"
 
 inline_for_extraction noextract
 val get_high_part: a:uint64 -> r:uint32{uint_v r == uint_v a / pow2 32}
@@ -25,6 +26,7 @@ let get_high_part a = to_u32 (shift_right a (size 32))
 inline_for_extraction noextract
 val get_low_part: a:uint64 -> r:uint32{uint_v r == uint_v a % pow2 32}
 let get_low_part a = to_u32 a
+
 
 val shift_bound: #n:nat -> num:UInt.uint_t n -> n':nat ->
   Lemma (num * pow2 n' <= pow2 (n' + n) - pow2 n')
@@ -88,35 +90,17 @@ let lemma_xor_zero l h =
   logxor_spec l h
 
 
+inline_for_extraction noextract
 val store_high_low_u: high:uint32 -> low:uint32 -> r:uint64{v r = v high * pow2 32 + v low}
-
 let store_high_low_u high low =
-  let as_uint64_high = to_u64 high in
-  let as_uint64_high = Lib.IntTypes.shift_left as_uint64_high (size 32) in
-  let as_uint64_low = to_u64 low in
+  [@inline_let] let as_uint64_high = Lib.IntTypes.shift_left (to_u64 high) (size 32) in
+  [@inline_let] let as_uint64_low = to_u64 low in
   assert (v as_uint64_high = v high * pow2 32);
   assert (v as_uint64_low = v low);
   lemma_xor_zero as_uint64_low as_uint64_high;
   logxor as_uint64_low as_uint64_high
 
 #push-options "--z3rlimit 100"
-
-inline_for_extraction noextract
-val load_buffer: a0: uint64 -> a1: uint64 -> a2: uint64 -> a3: uint64
-  -> o: lbuffer uint64 (size 4)
-  -> Stack unit
-    (requires fun h -> live h o)
-    (ensures  fun h0 _ h1 ->
-       modifies (loc o) h0 h1 /\
-       as_nat h1 o = v a0 + v a1 * pow2 64 + v a2 * pow2 128 + v a3 * pow2 192)
-
-let load_buffer a0 a1 a2 a3 o =
-  assert_norm (pow2 64 * pow2 64 = pow2 128);
-  assert_norm (pow2 64 * pow2 64 * pow2 64 = pow2 192);
-  upd o (size 0) a0;
-  upd o (size 1) a1;
-  upd o (size 2) a2;
-  upd o (size 3) a3
 
 inline_for_extraction noextract
 val upl_zer_buffer:
@@ -146,7 +130,7 @@ let upl_zer_buffer c0 c1 c2 c3 c4 c5 c6 c7 o =
     assert(v b2 = v c5 * pow2 32 + v c4);
     assert(v b3 = v c7 * pow2 32 + v c6);
 
-    load_buffer b0 b1 b2 b3 o;
+    bn_make_u64_4 b0 b1 b2 b3 o;
     fmod_short o o;
     let h2 = ST.get() in
     assert(as_nat h2 o = (v c1 * pow2 32 + v c0 + v c3 * pow2 (3 * 32) + v c2 * pow2 (2 * 32) + v c5 * pow2 (32 * 5) + v c4 * pow2 (32 * 4) + v c7 * pow2 (32 * 7) + v c6 * pow2 (32 * 6)) % prime256)
@@ -171,7 +155,7 @@ let upl_fir_buffer c11 c12 c13 c14 c15 o =
   let b1 = store_high_low_u c11 (u32 0) in
   let b2 = store_high_low_u c13 c12 in
   let b3 = store_high_low_u c15 c14 in
-  load_buffer b0 b1 b2 b3 o;
+  bn_make_u64_4 b0 b1 b2 b3 o;
   fmod_short o o
 
 inline_for_extraction noextract
@@ -181,7 +165,7 @@ val upl_sec_buffer: c12: uint32 -> c13: uint32 -> c14: uint32 -> c15: uint32
     (requires fun h -> live h o)
     (ensures fun h0 _ h1 ->
       modifies (loc o) h0 h1 /\
-      as_nat h1 o == (v c12 * pow2 (3 * 32) + v c13 * pow2 (4 * 32) + v c14 * pow2 (5 * 32) + v c15 * pow2 (6 * 32)) % prime /\ as_nat h1 o < prime
+      as_nat h1 o == (v c12 * pow2 (3 * 32) + v c13 * pow2 (4 * 32) + v c14 * pow2 (5 * 32) + v c15 * pow2 (6 * 32)) % prime256 /\ as_nat h1 o < prime256
     )
 
 let upl_sec_buffer c12 c13 c14 c15 o =
@@ -194,10 +178,10 @@ let upl_sec_buffer c12 c13 c14 c15 o =
     let b1 = store_high_low_u c12 (u32 0) in
     let b2 = store_high_low_u c14 c13 in
     let b3 = store_high_low_u (u32 0) c15 in
-    load_buffer b0 b1 b2 b3 o;
-    assert_norm(v c12 * pow2 (3 * 32) + v c13 * pow2 (4 * 32) + v c14 * pow2 (5 * 32) + v c15 * pow2 (6 * 32) < prime);
+    bn_make_u64_4 b0 b1 b2 b3 o;
+    assert_norm(v c12 * pow2 (3 * 32) + v c13 * pow2 (4 * 32) + v c14 * pow2 (5 * 32) + v c15 * pow2 (6 * 32) < prime256);
     let h1 = ST.get() in
-    modulo_lemma (as_nat h1 o) prime
+    FStar.Math.Lemmas.modulo_lemma (as_nat h1 o) prime256
 
 inline_for_extraction noextract
 val upl_thi_buffer: c8: uint32 -> c9: uint32 -> c10: uint32 -> c14: uint32 -> c15: uint32
@@ -217,7 +201,7 @@ let upl_thi_buffer c8 c9 c10 c14 c15 o =
    let b1 = store_high_low_u (u32 0) c10 in
    let b2 = u64 0 in
    let b3 = store_high_low_u c15 c14 in
-   load_buffer b0 b1 b2 b3 o;
+   bn_make_u64_4 b0 b1 b2 b3 o;
    fmod_short o o
 
 inline_for_extraction noextract
@@ -238,7 +222,7 @@ let upl_for_buffer c8 c9 c10 c11 c13 c14 c15 o =
   let b1 = store_high_low_u c13 c11 in
   let b2 = store_high_low_u c15 c14 in
   let b3 = store_high_low_u c8 c13 in
-  load_buffer b0 b1 b2 b3 o;
+  bn_make_u64_4 b0 b1 b2 b3 o;
   fmod_short o o
 
 inline_for_extraction noextract
@@ -259,7 +243,7 @@ let upl_fif_buffer c8 c10 c11 c12 c13 o =
     let b1 = store_high_low_u (u32 0) c13 in
     let b2 = u64 0 in
     let b3 = store_high_low_u c10 c8 in
-    load_buffer b0 b1 b2 b3 o;
+    bn_make_u64_4 b0 b1 b2 b3 o;
     fmod_short o o
 
 inline_for_extraction noextract
@@ -281,7 +265,7 @@ let upl_six_buffer c9 c11 c12 c13 c14 c15 o =
     let b1 = store_high_low_u c15 c14 in
     let b2 = u64 0 in
     let b3 = store_high_low_u c11 c9 in
-    load_buffer b0 b1 b2 b3 o;
+    bn_make_u64_4 b0 b1 b2 b3 o;
     fmod_short o o
 
 inline_for_extraction noextract
@@ -303,7 +287,7 @@ let upl_sev_buffer c8 c9 c10 c12 c13 c14 c15 o =
     let b1 = store_high_low_u c8 c15 in
     let b2 = store_high_low_u c10 c9 in
     let b3 = store_high_low_u c12 (u32 0) in
-    load_buffer b0 b1 b2 b3 o;
+    bn_make_u64_4 b0 b1 b2 b3 o;
     fmod_short o o
 
 inline_for_extraction noextract
@@ -324,7 +308,7 @@ let upl_eig_buffer c9 c10 c11 c12 c13 c14 c15 o =
     let b1 = store_high_low_u c9 (u32 0) in
     let b2 = store_high_low_u c11 c10 in
     let b3 = store_high_low_u c13 (u32 0) in
-    load_buffer b0 b1 b2 b3 o;
+    bn_make_u64_4 b0 b1 b2 b3 o;
     fmod_short o o
 
 
@@ -343,16 +327,16 @@ val solinas_reduction_upload: c0: uint32 -> c1: uint32 -> c2: uint32 -> c3: uint
           let t6 = as_nat h1 (gsub tempBuffer (size 24) (size 4)) in
           let t7 = as_nat h1 (gsub tempBuffer (size 28) (size 4)) in
           let t8 = as_nat h1 (gsub tempBuffer (size 32) (size 4)) in
-          t0 == (v c0 + v c1 * pow2 (1 * 32) + v c2 * pow2 (2 * 32) + v c3 * pow2 (3 * 32) + v c4 * pow2 (4 * 32) + v c5 * pow2 (5 * 32) + v  c6 * pow2 (6 * 32) +  v c7 * pow2 (7 * 32)) % prime /\
+          t0 == (v c0 + v c1 * pow2 (1 * 32) + v c2 * pow2 (2 * 32) + v c3 * pow2 (3 * 32) + v c4 * pow2 (4 * 32) + v c5 * pow2 (5 * 32) + v  c6 * pow2 (6 * 32) +  v c7 * pow2 (7 * 32)) % prime256 /\
           t1 == (v c11 * pow2 (3 * 32) + v c12 * pow2 (4 * 32) + v c13 * pow2 (5 * 32) +
-           v c14 * pow2 (6 * 32) + v c15 * pow2 (7 * 32)) % prime /\
-          t2 == (v c12 * pow2 (3 * 32) + v c13 * pow2 (4 * 32) +  v c14 * pow2 (5 * 32) + v c15 * pow2 (6 * 32)) % prime  /\
-          t3 == (v c8 + v c9 * pow2 32 + v c10 * pow2 (2 * 32) + v c14 * pow2 (6 * 32) + v c15 * pow2 (7 * 32)) % prime /\
-          t4 == (v c9 + v c10 * pow2 32 + v c11 * pow2 (2 * 32) + v c13 * pow2 (3 * 32) + v c14 * pow2 (4 * 32) + v c15 * pow2 (5 * 32) + v c13 * pow2 (6 * 32) + v c8 * pow2 (7 * 32)) % prime /\
-          t5 == (v c11 + v c12 * pow2 32 + v c13 * pow2 (2 * 32) + v c8 * pow2 (6 * 32) + v c10 * pow2 (7 * 32)) % prime /\
-          t6 == (v c12 + v c13 * pow2 32 + v c14 * pow2 (2 * 32) + v c15 * pow2 (3 * 32) + v c9 * pow2 (6 * 32) + v c11 * pow2 (7 * 32)) % prime /\
-          t7 == (v c13 + v c14 * pow2 32 + v c15 * pow2 (2 * 32) +  v c8 * pow2 (3 * 32) +  v c9 * pow2 (4 * 32) + v c10 * pow2 (5 * 32) + v c12 * pow2 (7 * 32)) % prime /\
-          t8 == (v c14 + v c15 * pow2 32 + v c9 * pow2 (3 * 32) +  v c10 * pow2 (4 * 32) + v c11 * pow2 (5 * 32) + v c13 * pow2 (7 * 32)) % prime
+           v c14 * pow2 (6 * 32) + v c15 * pow2 (7 * 32)) % prime256 /\
+          t2 == (v c12 * pow2 (3 * 32) + v c13 * pow2 (4 * 32) +  v c14 * pow2 (5 * 32) + v c15 * pow2 (6 * 32)) % prime256  /\
+          t3 == (v c8 + v c9 * pow2 32 + v c10 * pow2 (2 * 32) + v c14 * pow2 (6 * 32) + v c15 * pow2 (7 * 32)) % prime256 /\
+          t4 == (v c9 + v c10 * pow2 32 + v c11 * pow2 (2 * 32) + v c13 * pow2 (3 * 32) + v c14 * pow2 (4 * 32) + v c15 * pow2 (5 * 32) + v c13 * pow2 (6 * 32) + v c8 * pow2 (7 * 32)) % prime256 /\
+          t5 == (v c11 + v c12 * pow2 32 + v c13 * pow2 (2 * 32) + v c8 * pow2 (6 * 32) + v c10 * pow2 (7 * 32)) % prime256 /\
+          t6 == (v c12 + v c13 * pow2 32 + v c14 * pow2 (2 * 32) + v c15 * pow2 (3 * 32) + v c9 * pow2 (6 * 32) + v c11 * pow2 (7 * 32)) % prime256 /\
+          t7 == (v c13 + v c14 * pow2 32 + v c15 * pow2 (2 * 32) +  v c8 * pow2 (3 * 32) +  v c9 * pow2 (4 * 32) + v c10 * pow2 (5 * 32) + v c12 * pow2 (7 * 32)) % prime256 /\
+          t8 == (v c14 + v c15 * pow2 32 + v c9 * pow2 (3 * 32) +  v c10 * pow2 (4 * 32) + v c11 * pow2 (5 * 32) + v c13 * pow2 (7 * 32)) % prime256
     ))
 
 
@@ -391,8 +375,8 @@ val solinas_reduction_operations: tempBuffer: lbuffer uint64 (size 36) ->  o: lb
           let t6 = as_nat h (gsub tempBuffer (size 24) (size 4)) in
           let t7 = as_nat h (gsub tempBuffer (size 28) (size 4)) in
           let t8 = as_nat h (gsub tempBuffer (size 32) (size 4)) in
-          t0 < prime /\ t1 < prime /\ t2 < prime /\ t3 < prime /\ t4 < prime /\
-          t5 < prime /\ t6 < prime /\ t7 < prime /\ t8 < prime
+          t0 < prime256 /\ t1 < prime256 /\ t2 < prime256 /\ t3 < prime256 /\ t4 < prime256 /\
+          t5 < prime256 /\ t6 < prime256 /\ t7 < prime256 /\ t8 < prime256
       )
     )
     (ensures fun h0 _ h1 -> modifies2 tempBuffer o h0 h1 /\
@@ -406,7 +390,7 @@ val solinas_reduction_operations: tempBuffer: lbuffer uint64 (size 36) ->  o: lb
           let t6 = as_nat h0 (gsub tempBuffer (size 24) (size 4)) in
           let t7 = as_nat h0 (gsub tempBuffer (size 28) (size 4)) in
           let t8 = as_nat h0 (gsub tempBuffer (size 32) (size 4)) in
-          as_nat h1 o == (t0 + 2 * t1 + 2 * t2  + t3 + t4 - t5  - t6 - t7 - t8) % prime
+          as_nat h1 o == (t0 + 2 * t1 + 2 * t2  + t3 + t4 - t5  - t6 - t7 - t8) % prime256
     )
   )
 
@@ -465,7 +449,7 @@ val lemma_opened: i:Lib.Sequence.lseq uint64 8 -> Lemma
    let c14 = get_low_part  i7 in
    let c15 = get_high_part i7 in
 
-   felem_seq_as_nat_8 i =
+   felem_wide_seq_as_nat i =
      v c0  * pow2 (0 * 32) +
      v c1  * pow2 (1 * 32) +
      v c2  * pow2 (2 * 32) +
@@ -486,6 +470,7 @@ val lemma_opened: i:Lib.Sequence.lseq uint64 8 -> Lemma
 #push-options "--z3rlimit 400"
 
 let lemma_opened i =
+  let open FStar.Math.Lemmas in
   let open Lib.Sequence in
 
   let i0 = index i 0 in
@@ -602,7 +587,7 @@ let lemma_opened i =
   };
 
   calc (==) {
-    felem_seq_as_nat_8 i;
+    felem_wide_seq_as_nat i;
     == { }
     v i0 * pow2 (0 * 64) +
     v i1 * pow2 (1 * 64) +
@@ -641,6 +626,7 @@ let lemma_opened i =
   }
 
 
+[@CInline]
 let solinas_reduction_impl i o =
   push_frame();
 
@@ -692,5 +678,5 @@ let solinas_reduction_impl i o =
 
     solinas_reduction_mod (v c0) (v c1) (v c2) (v c3) (v c4) (v c5) (v c6) (v c7) (v c8) (v c9) (v c10) (v c11) (v c12) (v c13) (v c14) (v c15) (as_nat h1 t0) (as_nat h1 t1) (as_nat h1 t2) (as_nat h1 t3) (as_nat h1 t4) (as_nat h1 t5) (as_nat h1 t6) (as_nat h1 t7) (as_nat h1 t8) (as_nat h2 o);
 
-  modulo_lemma (as_nat h2 o) prime;
+  FStar.Math.Lemmas.modulo_lemma (as_nat h2 o) prime;
   pop_frame()
