code/ecdsap256/Hacl.Impl.P256.SolinasReduction.fsti
@@ -9,11 +9,11 @@ open Lib.Buffer
 
 open Spec.P256.Constants
 open Hacl.Spec.P256.Felem
-open Hacl.Spec.P256.SolinasReduction.Lemmas
 
 #set-options "--z3rlimit 30 --fuel 0 --ifuel 0"
 
-val solinas_reduction_impl: i: lbuffer uint64 (size 8) -> o: lbuffer uint64 (size 4) ->
+val solinas_reduction_impl: f:lbuffer uint64 (size 8) -> res:lbuffer uint64 (size 4) ->
   Stack unit
-    (requires fun h -> live h i /\ live h o /\ disjoint i o)
-    (ensures fun h0 _ h1 -> modifies1 o h0 h1 /\ wide_as_nat h0 i % prime == as_nat h1 o)
+  (requires fun h -> live h f /\ live h res /\ disjoint f res)
+  (ensures fun h0 _ h1 -> modifies1 res h0 h1 /\
+    as_nat h1 res == wide_as_nat h0 f % prime256)
